---
layout: post
title: A Proof of Jensen's Inequality and its Applications
categories: [Mathematics, Analysis]
use_math: true
---
The proofs for Jensen's inequality are motivated by Exercise 8.9 in *Real Analysis for Graduate Students* by Richard F. Bass.

**Definition 1** A function $f : \mathbb{R} \rightarrow \mathbb{R}$ is *convex* if

$$\begin{aligned}
f(\lambda x + (1 - \lambda) y) \leq \lambda f(x) + (1 - \lambda) f(y)
\end{aligned}$$

whenever $x < y \in \mathbb{R}$ and $\lambda \in [0,1]$.

**Definition 2** A *subderivative* of a convex function $f : \mathbb{R} \rightarrow \mathbb{R}$ at a point $x_0$ is a real number $c$ such that
\begin{align}
f(x) \geq f(x_0) + c(x - x_0)
\end{align}
for all $x \in \mathbb{R}$.

**Proposition 3** A subderivative of a convex function $f : \mathbb{R} \rightarrow \mathbb{R}$ always exists at any point $x_0$.

*Proof.* Let $x < y < z \in \mathbb{R}$ be given. First notice that $y = \lambda x + (1 - \lambda) z$ where

$$\begin{aligned}
\lambda = \frac{y - z}{x - z} \in (0,1).
\end{aligned}$$

Then since $f$ is convex,

$$\begin{aligned}
f(y) \leq \left( \frac{y - z}{x - z} \right) f(x) + \left( \frac{x - y}{x - z} \right) f(y)
\end{aligned}$$

which implies

$$\begin{aligned}
\frac{f(x) - f(y)}{x - y} \leq \frac{f(z) - f(y)}{z - y}.
\end{aligned}$$

Hence the interval

$$\begin{aligned}
\partial f(x_0) \mathrel{:=} \left[ \limsup_{h \rightarrow 0} \frac{f(x_0 - h) - f(x_0)}{-h}, \ \liminf_{h \rightarrow 0} \frac{f(x_0 + h) - f(x_0)}{h} \right]
\end{aligned}$$

is nonempty, and we can choose $c \in \partial f(x_0)$. Let an arbitrary $x \in \mathbb{R}$ be given. If $x = x_0$, Inequality (1) is trivially satisfied. If $x < x_0$,

$$\begin{aligned}
\frac{f(x) - f(x_0)}{x - x_0} \leq \limsup_{h \rightarrow 0} \frac{f(x_0 - h) - f(x)}{-h} \leq c
\end{aligned}$$

and thus Inequality (1) is satisfied. If $x > x_0$,

$$\begin{aligned}
\frac{f(x) - f(x_0)}{x - x_0} \geq \liminf_{h \rightarrow 0} \frac{f(x_0 + h) - f(x_0)}{h} \geq c
\end{aligned}$$

and again Inequality (1) is satisfied. This completes the proof. $$\tag*{$\blacksquare$}$$

**Theorem 4** (Jensen's Inequality) Let $(X,\mathcal{A},\mu)$ be a measure space, suppose $\mu(X) = 1$, and let $f : \mathbb{R} \rightarrow \mathbb{R}$ be convex. Then the following inequality holds:

$$\begin{aligned}
f \left( \int g \, d\mu \right) \leq \int f \circ g \, d\mu.
\end{aligned}$$

*Proof.* Let $x_0 = \int g$. By Proposition 3, there is $c \in \mathbb{R}$ such that $f(y) \geq f(x_0) + c(y - x_0)$ for all $y \in \mathbb{R}$. Hence

$$\begin{aligned}
\int f \circ g \, d\mu &\geq \int (f(x_0) + c(g(x) - x_0)) \, d\mu \\
&= \mu(X) f(x_0) + c \int g \, d\mu - c x_0 \mu(X) \\
&= f(x_0) = f \left( \int g \, d\mu \right).
\end{aligned}$$

$$\tag*{$\blacksquare$}$$
